ListEmbedding

common/JWordList.ec
@@ -3,115 +3,999 @@ require import AllCore List Int IntDiv.
 from Jasmin require import JMemory JWord JUtils.
 
 
-require import EclibExtra.
+(*from JazzCommon*) require import EclibExtra.
+require BitEncoding.
+import BitEncoding.BitChunking.
+require import StdOrder.
+import IntOrder.
 
+
+(* TO JUtils *)
+(* MOVE THIS!!! *)
+lemma map2_nilr ['a, 'b, 'c] (f : 'a -> 'b -> 'c) l:
+ map2 f l [] = [].
+proof.
+rewrite -size_eq0 size_map2 /=; smt(size_ge0).
+qed.
+
+lemma map2_nill ['a, 'b, 'c] (f : 'a -> 'b -> 'c) l:
+ map2 f [] l = [].
+proof.
+rewrite -size_eq0 size_map2 /=; smt(size_ge0).
+qed.
+
+(* a more general version *)
+lemma nth_map' ['a 'b] (da: 'a) (f: 'a -> 'b) (l: 'a list) db i:
+ f da = db =>
+ nth db (map f l) i = f (nth da l i).
+proof.
+move => Hf.
+case: (0 <= i && i < size l) => C.
+ by rewrite (nth_map da) //.
+by rewrite !nth_out; smt(size_map).
+qed.
+
+(* TO JWord *)
+lemma W8_bits2w_nil:
+ W8.bits2w [] = W8.zero.
+proof. by apply W8.ext_eq => i Hi; rewrite /bits2w initiE //=. qed.
+
+(* slightly more general version of W8.bits2K *)
+lemma W8_bits2wK' l:
+ size l <= 8 =>
+ W8.w2bits (W8.bits2w l) = l ++ nseq (8 - size l) false.
+proof.
+move=> H; apply (eq_from_nth false).
+ by rewrite size_w2bits size_cat size_nseq; smt(size_ge0).
+move=> i; rewrite size_w2bits => Hi.
+rewrite get_w2bits get_bits2w 1:// nth_cat.
+case: (i < size l) => C //.
+case: ((i - size l) < (8 - size l)) => C2.
+ by rewrite !nth_nseq 1:/# nth_out /#.
+smt(nth_out).
+qed.
+
+lemma W8_bits2w_cat_nseq0 bs n:
+ W8.bits2w (bs ++ nseq n false)
+ = W8.bits2w bs.
+proof.
+apply W8.ext_eq => i Hi.
+rewrite /bits2w !initiE //= nth_cat.
+case: (i < size bs) => C //.
+rewrite !nth_nseq_if nth_out; smt(size_ge0).
+qed.
+
+lemma W64_bits2w_nil:
+ W64.bits2w [] = W64.zero.
+proof. by apply W64.ext_eq => i Hi; rewrite /bits2w initiE //=. qed.
+
+lemma W64_bits2wK' l:
+ size l <= 64 =>
+ W64.w2bits (W64.bits2w l) = l ++ nseq (64 - size l) false.
+proof.
+move=> H; apply (eq_from_nth false).
+ by rewrite size_w2bits size_cat size_nseq; smt(size_ge0).
+move=> i; rewrite size_w2bits => Hi.
+rewrite get_w2bits get_bits2w 1:// nth_cat.
+case: (i < size l) => C //.
+case: ((i - size l) < (64 - size l)) => C2.
+ by rewrite !nth_nseq 1:/# nth_out /#.
+smt(nth_out).
+qed.
+
+lemma W64_bits2w_cat_nseq0 bs n:
+ W64.bits2w (bs ++ nseq n false)
+ = W64.bits2w bs.
+proof.
+apply W64.ext_eq => i Hi.
+rewrite /bits2w !initiE //= nth_cat.
+case: (i < size bs) => C //.
+rewrite !nth_nseq_if nth_out; smt(size_ge0).
+qed.
+
+lemma W8u8_to_listK w: pack8 (W8u8.to_list w) = w.
+proof.
+apply W64.ext_eq => k Hk.
+rewrite -(W8u8.unpack8K w); congr; congr.
+rewrite of_listE unpack8E; apply W8u8.Pack.all_eq_eq.
+by rewrite /all_eq /=.
+qed.
+
+lemma W8u8_to_list_pack8 l: 
+ size l <= 8 => W8u8.to_list (W8u8.pack8 l) = l ++ nseq (8-size l) W8.zero.
+proof.
+move=> Hl; apply (eq_from_nth W8.zero).
+ by rewrite /= size_cat size_nseq /#.
+move => i Hi; rewrite /= in Hi.
+have: (i \in iotared 0 8) by smt().
+move: {Hi} i; rewrite -allP /=.
+rewrite !W8u8.pack8bE // !get_of_list //.
+by rewrite !nth_cat; smt(nth_nseq nth_out).
+qed.
+
+lemma W8u8_pack8_nil: W8u8.pack8 [] = W64.zero.
+proof.
+apply W64.ext_eq => k Hk.
+by rewrite pack8E initiE //= get_of_list 1:/# /=.
+qed.
+
+
+
+lemma W8u8_to_listE (w: W64.t):
+ W8u8.to_list w = W8u8.Pack.to_list (unpack8 w).
+proof.
+by rewrite W8u8.unpack8E W8u8.Pack.to_listE /mkseq -iotaredE /=.
+qed.
+
+lemma W8u8_unpack8_inj: injective W8u8.unpack8.
+proof.
+move=> w1 w2.
+rewrite !unpack8E => E.
+apply W64.ext_eq => k Hk.
+rewrite !get_bits8 1..2://; congr.
+have /= <-:= W8u8.Pack.initiE (fun (i : int) => w1 \bits8 i) (k%/8) _.
+ smt().
+by rewrite E W8u8.Pack.initiE /#.
+qed.
+
+lemma W8u8_to_list_inj:
+ injective W8u8.to_list.
+proof.
+by move=> w1 w2; rewrite !W8u8_to_listE => /W8u8.Pack.to_list_inj /W8u8_unpack8_inj.
+qed.
+
+(** sets a specific byte of a 64-bit word *)
+op w64_set_u8 (w:W64.t, pos: int, x: W8.t): W64.t =
+ pack8_t (unpack8 w).[pos <- x].
+
+op w64_xor_u8 (w: W64.t, pos: int, x: W8.t): W64.t =
+ let w8u8 = unpack8 w in pack8_t w8u8.[pos <- w8u8.[pos] `^` x].
+
+(* end JWord*)
+
+
+lemma map_chunkK ['a] (f:'a list -> 'a list) n bs:
+ 0 < n =>
+ n %| size bs =>
+ (forall l, size l=n => f l = l) =>
+ flatten (map f (chunk n bs)) = bs.
+proof.
+move => Hn Hsz Hf.
+have [E _]:= (eq_in_map f idfun (chunk n bs)).
+rewrite E.
+ move=> x Hx; rewrite Hf //.
+ by rewrite (in_chunk_size n bs) //.
+by rewrite map_id chunkK //.
+qed.
+
+
+op chunkremains ['a] n (bs: 'a list) =
+ drop (size bs %/ n * n) bs.
+
+lemma size_chunkremains ['a] n (bs: 'a list):
+ size (chunkremains n bs) = size bs %% n.
+proof.
+rewrite size_drop. smt(size_ge0).
+rewrite lez_maxr; first smt(size_ge0).
+by rewrite {1}(divz_eq (size bs) n) /#.
+qed.
+
+(** An "extended" version of [chunkK] *)
+lemma chunkK' ['a] r (bs: 'a list):
+ 0 < r =>
+ flatten (chunk r bs) ++ chunkremains r bs
+ = bs.
+proof.
+move=> Hr; rewrite chunk_take_eq //.
+rewrite chunkK //.
+ rewrite size_take; first smt(size_ge0).
+ rewrite {2}(divz_eq (size bs) r).
+ case: (size bs %% r = 0)=> C; first smt().
+ rewrite ifT 1:/#.
+ by rewrite dvdz_mull /#.
+by rewrite cat_take_drop.
+qed.
+
+lemma chunk_cat' ['a] (l1 l2: 'a list) r:
+ 0 < r =>
+ chunk r (l1++l2)
+ = chunk r l1 ++ chunk r (chunkremains r l1 ++ l2).
+proof.
+move=> Hr.
+rewrite -{1}(cat_take_drop (size l1 %/ r * r) l1) -catA chunk_cat.
+ rewrite size_take; first smt(size_ge0).
+ rewrite {2}(divz_eq (size l1) r).
+ case: (size l1 %% r = 0)=> C; first smt().
+ rewrite ifT 1:/#.
+ by rewrite dvdz_mull /#.
+by rewrite -chunk_take_eq //.
+qed.
+
+lemma chunk0 ['a] n (l: 'a list):
+ size l < n =>
+ chunk n l = [].
+proof.
+move=> Hl; rewrite /chunk divz_small; smt(size_ge0 mkseq0).
+qed.
+
+lemma chunk1 ['a] r (l: 'a list):
+ 0 < r =>
+ size l = r =>
+ chunk r l = [l].
+proof.
+move=> Hr Hsz; rewrite /chunk Hsz divzz (:r<>0) 1:/# b2i1 /=.
+by rewrite /mkseq -iotaredE /= drop0 -Hsz take_size.
+qed.
+
+(** [chunkpad] used to zero-fill the last chunk *)
+op chunkpad ['a] (d:'a) r (l: 'a list) =
+ nseq ((-size l)%%r) d.
+
+lemma chunkpad_nil ['a] (d: 'a) r:
+ chunkpad d r [] = [].
+proof. by rewrite /chunkpad /= nseq0. qed.
+
+lemma chunkpadE ['a] (d: 'a) r l:
+ 0 < r => 
+ chunkpad d r l = if r %| size l then [] else nseq (r - size l %% r) d.
+proof.
+move=> Hr. 
+case: (r %| size l) => [/dvdzE|] C.
+ by rewrite /chunkpad /= -modzNm C /= nseq0.
+by rewrite /chunkpad /= -modzNm -modzDl modz_small /#.
+qed.
+
+lemma size_chunkpad ['a] (d: 'a) r l:
+ 0 < r =>
+ size (chunkpad d r l) = b2i (! r %| size l) * (r - size l %% r).
+proof.
+move=> Hr.
+case: (r %| size l) => [/dvdzE|] C.
+ by rewrite /chunkpad /size_cat size_nseq ler_maxr 1:/# b2i0 -modzNm C.
+by rewrite b2i1 chunkpadE // C /= size_nseq /#.
+qed.
+
+(** [chunkfill] zero-fills the last chunk *)
+op chunkfill ['a] (d: 'a) r l =
+ l ++ chunkpad d r l.
+
+lemma size_chunkfill ['a] (d: 'a) r l:
+ 0 < r =>
+ size (chunkfill d r l) = size l %/ r * r + b2i (! r %| size l) * r.
+proof.
+move=> Hr; rewrite /chunkfill size_cat size_chunkpad //.
+case: (r %| size l) => C /=.
+ by rewrite b2i0 /= divzK.
+by rewrite b2i1 {1}(divz_eq (size l) r) /#.
+qed.
+
+lemma chunkfill_nil ['a] (d: 'a) r:
+ chunkfill d r [] = [].
+proof. by rewrite /chunkfill /chunkpad /= nseq0. qed.
+
+lemma chunkfillP ['a] (d: 'a) r l:
+ 0 < r =>
+ r %| size (chunkfill d r l).
+proof.
+move=> Hr; rewrite size_chunkfill //.
+case: (r %| size l) => C /=; first smt().
+by rewrite b2i1 /= dvdzD /#.
+qed.
+
+lemma chunkfillE ['a] (d: 'a) r l:
+ 0 < r =>
+ chunkfill d r l = if r %| size l then l else l ++ chunkpad d r l.
+proof.
+move=> Hr; rewrite /chunkfill chunkpadE //; smt(cats0).
+qed.
+
+(** [chunkify] is a version of [chunk] that allows the existence
+ of an incomplete chunk at the end of the list *)
+(*
+op chunkify ['a] d r (bs: 'a list) =
+ chunk r (chunkfill d r bs).
+*)
+op chunkify ['a] r (bs: 'a list) =
+ mkseq (fun (i : int) => take r (drop (r * i) bs))
+       (size bs %/ r + b2i (! r %| size bs)).
+
+lemma chunkifyE ['a] r (bs: 'a list):
+ 0 < r =>
+ chunkify r bs
+ = chunk r bs ++ if r %| size bs then [] else [chunkremains r bs].
+proof.
+move=> Hr; rewrite /chunkify; case: (r %| size bs) => C.
+ by rewrite b2i0 cats0.
+rewrite b2i1 mkseqS; first smt(size_ge0).
+rewrite cats1; congr => //=.
+rewrite /chunkremains take_oversize.
+ by rewrite size_drop; smt(size_ge0).
+by rewrite mulrC.
+qed.
+
+lemma chunkify_chunk ['a] n (bs: 'a list):
+ 0 < n =>
+ n %| size bs =>
+ chunkify n bs = chunk n bs.
+proof.
+move=> Hn Hsz.
+by rewrite chunkifyE // Hsz /= cats0.
+qed.
+
+lemma chunkify_cat ['a] n (l1 l2: 'a list):
+ 0 < n =>
+ n %| size l1 =>
+ chunkify n (l1++l2) = chunkify n l1 ++ chunkify n l2.
+proof.
+move => Hn Hsz.
+rewrite (chunkify_chunk _ l1) // chunkifyE // chunk_cat // -!catA; congr.
+rewrite chunkifyE; case: (n %| size l2) => // C.
+ rewrite size_cat ifT /= ?cats0 //; smt(dvdzD).
+ rewrite size_cat.
+ rewrite ifF.
+ move: C; apply contra; smt(dvdzB).
+rewrite /chunkremains size_cat; congr.
+have ->: (size l1 + size l2)%/ n * n
+         = size l1 + size l2 %/ n * n.
+ by rewrite divzDl // /#.
+by rewrite drop_cat ifF; smt(size_ge0).
+qed.
+
+lemma chunkify_nil ['a] n: chunkify <:'a> n [] = [].
+by rewrite /chunkify mkseq0. qed.
+
+lemma chunkify_cons ['a] n (l: 'a list):
+ 0 < n =>
+ 0 < size l =>
+ chunkify n l = take n l :: chunkify n (drop n l).
+proof.
+move => n_gt0 Hsz0.
+ rewrite -{1}(cat_take_drop n l).
+case: (size l < n) => Hsz.
+ by rewrite !drop_oversize 1:/# cats0 take_oversize 1:/# chunkify_nil chunkifyE // chunk0 /#.
+rewrite chunkify_cat ?size_take 1..3:/# chunkify_chunk // ?size_take' 1..2:/# chunk1 1:/#. 
+ by rewrite size_take' /#.
+smt().
+qed.
+
+lemma size_chunkify ['a] n (bs: 'a list):
+ 0 < n =>
+ size (chunkify n bs)
+ = size bs %/ n + b2i (! n %| size bs).
+proof.
+by move=> Hn; rewrite /chunkify size_mkseq; smt(size_ge0). 
+qed.
+
+lemma nth_chunkify ['a] n (bs: 'a list) (i: int):
+ 0 < n =>
+ 0 <= i =>
+ nth [] (chunkify n bs) i = take n (drop (n*i) bs).
+proof.
+move=> Hn Hi.
+case: (i < size bs %/ n + b2i (! n %| size bs)) => C.
+ by rewrite nth_mkseq //=.
+rewrite nth_out ?size_chunkify // 1:/#. 
+rewrite drop_oversize ?take_nil //.
+rewrite (divz_eq (size bs) n); move: C; case: (n %| size bs).
+ by rewrite b2i0 /= => /dvdzE -> C2 /#.
+by rewrite b2i1 /= => C1 C2 /#.
+qed.
+
+lemma take_chunkify ['a] n (bs: 'a list) k:
+ 0 < n =>
+ take k (chunkify n bs) = chunkify n (take (n*k) bs).
+proof.
+move=> n_gt0; rewrite -{1}(cat_take_drop (n*k) bs).
+case: (0 <= n*k) => Hsz0; last first. 
+ by rewrite !take_le0 1..2:/# /chunkify /= mkseq0_le //.
+case: (n*k <= size bs) => E.
+ rewrite chunkify_cat //.
+  by rewrite size_take' 1:/# E /= dvdz_mulr dvdzz. 
+ rewrite take_cat' !size_chunkify // size_take' // !E /= ifT. 
+  by rewrite (:n %| n * k); smt(dvdz_mulr dvdzz). 
+ rewrite take_oversize // size_chunkify // !size_take' // E /=.
+ by rewrite dvdz_mulr ?dvdzz /= b2i0 /#.
+rewrite drop_oversize 1:/# cats0 take_oversize //.
+by rewrite size_chunkify // size_take' /#.
+qed.
+
+lemma drop_chunkify ['a] n (bs: 'a list) k:
+ 0 < n =>
+ drop k (chunkify n bs) = chunkify n (drop (n*k) bs).
+proof.
+move => n_gt0; elim/natind: k bs => //=.
+ by move=> k Hk l; rewrite !drop_le0 // /#.
+move=> k Hk IH l.
+rewrite -drop_drop //.
+move: l => [|x xs] //.
+ by rewrite /chunkify //= mkseq0_le.
+rewrite {1}(chunkify_cons _ (x::xs) _) /= 1:/#; first smt(size_ge0).
+rewrite drop0 (:! n * (k + 1) <= 0) 1:/# /= IH ifF 1:/# drop_drop 1..2:/#.
+by congr; congr; ring.
+qed.
+
+(** an alternative definition (normally not as usefull) for
+ the size of chunkify *)
+lemma sizechunkifyE n bslen:
+ 0 < n =>
+ 0 <= bslen =>
+ bslen %/ n + b2i (! n %| bslen)
+ = (bslen - 1) %/ n + 1.
+proof.
+move=> Hn Hsz.
+case: (n %| bslen) => [/dvdzE C|C].
+ by rewrite b2i0 /= /#.
+by rewrite divz_minus1 //.
+qed.
+
+(*
+(** [chunkfill] - zero-fill of a (partial) chunk *)
+op chunkfill ['a] (d: 'a) n bs =
+ take n (bs ++ nseq n d). 
+
+lemma chunkfillE ['a] (d: 'a) n bs:
+ chunkfill d n bs = if size bs < n then bs ++ nseq (n-size bs) d else take n bs.
+proof.
+rewrite /chunkfill; case: (size bs < n) => C.
+ by rewrite take_cat' ifF 1:/# take_nseq ler_minl; smt(size_ge0).
+by rewrite take_cat' ifT 1:/#.
+qed.
+
+lemma size_chunkfill ['a] (d: 'a) n bs:
+ 0 < n =>
+ size (chunkfill d n bs) = n.
+proof.
+by move=> Hn; rewrite /chunkfill size_take' 1:/# !size_cat size_nseq ifT; smt(size_ge0).
+qed.
+
+(** [chunkify_fillsuffix] - zero-suffix that fills the last chunk *)
+op chunkify_fillsuffix ['a] (d:'a) n sz =
+ nseq (b2i (! n %| sz) * (n - sz %% n)) d.
+*)
+
+lemma map_chunkifyK ['a] d (f:'a list -> 'a list) n bs:
+ 0 < n =>
+ (forall l, size l<=n => f l = chunkfill d n l) =>
+ flatten (map f (chunkify n bs))
+ = chunkfill d n bs. (* bs ++ chunkify_fillsuffix d n (size bs).*)
+proof.
+move => Hn Hf; rewrite chunkifyE // chunkfillE // map_cat flatten_cat.
+case: (n %| size bs) => C /=.
+ rewrite flatten_nil cats0.
+ apply map_chunkK => //.
+ by move=> l Hl; rewrite Hf 1:/# chunkfillE // Hl dvdzz.
+admitted (*
+rewrite chunkpadE // C /=. (* b2i1 /= chunk_take_eq //.*)
+rewrite -{3}(cat_take_drop (size bs %/ n * n)) -catA; congr.
+ rewrite map_chunkK => //.
+  rewrite size_take; first smt(size_ge0).
+  rewrite {2}(divz_eq (size bs) n).
+  case: (size bs %% n = 0)=> ?; first smt().
+  rewrite ifT 1:/#.
+  by rewrite dvdz_mull /#.
+ by move=> l Hl; rewrite Hf 1:/# take_size_cat.
+rewrite /flatten /= cats0 Hf; first smt(size_chunkremains).
+rewrite take_cat ifF; first smt(size_chunkremains).
+congr; first smt().
+rewrite take_nseq size_chunkremains ler_minl; smt(size_ge0).
+qed.
+*).
+
+
+abstract theory ListEmbedding.
+
+(* instantiate this... *)
+type SSS.
+type TTT.
+op n: int.
+op dSSS: SSS.
+op dTTT: TTT.
+op SSS_to_TTTs: SSS -> TTT list.
+op SSS_from_TTTs: TTT list -> SSS.
+
+(* ...and provide these proofs *)
+axiom n_gt0: 0 < n.
+axiom size_SSS_to_TTTs x: size (SSS_to_TTTs x) = n.
+axiom SSS_to_TTTs_inj: injective SSS_to_TTTs.
+axiom SSS_to_TTTsK x: SSS_from_TTTs (SSS_to_TTTs x) = x.
+axiom SSS_to_TTTs_nil: SSS_to_TTTs dSSS = nseq n dTTT.
+axiom SSS_from_TTTsK l:
+ size l <= n =>
+ SSS_to_TTTs (SSS_from_TTTs l) = l ++ nseq (n-size l) dTTT.
+axiom SSS_from_TTTs_nil: SSS_from_TTTs [] = dSSS.
+
+(* list embeddings and some facts *)
+op SSSs_to_TTTs (l: SSS list): TTT list =
+ flatten (map SSS_to_TTTs l).
+op SSSs_from_TTTs (l: TTT list): SSS list =
+ map SSS_from_TTTs (chunkify n l).
+
+lemma SSSs_to_TTTs_nil: SSSs_to_TTTs [] = [] by done.
+
+lemma SSSs_to_TTTs_cons x xs:
+ SSSs_to_TTTs (x::xs)
+ = (SSS_to_TTTs x) ++ SSSs_to_TTTs xs by done.
+
+lemma SSSs_to_TTTs_cat l1 l2:
+ SSSs_to_TTTs (l1++l2)
+ = SSSs_to_TTTs l1 ++ SSSs_to_TTTs l2.
+proof. by elim: l1 => //= x xs IH; rewrite !SSSs_to_TTTs_cons IH catA. qed.
+
+lemma size_SSSs_to_TTTs l:
+ size (SSSs_to_TTTs l) = n*size l.
+proof.
+rewrite /SSSs_to_TTTs size_flatten -map_comp /(\o) /=.
+rewrite StdBigop.Bigint.sumzE.
+rewrite StdBigop.Bigint.BIA.big_mapT /(\o) /=.
+rewrite -(StdBigop.Bigint.BIA.eq_bigr _ (fun (x:SSS) => n)).
+ by move=> i /= _; rewrite size_SSS_to_TTTs.
+by rewrite StdBigop.Bigint.big_constz count_predT_eq.
+qed.
+
+lemma SSSs_to_TTTs_inj: injective SSSs_to_TTTs.
+proof.
+rewrite /SSSs_to_TTTs; elim.
+ move=> [|y ys] //=.
+ rewrite flatten_nil flatten_cons.
+ rewrite eq_sym -size_eq0 size_cat size_SSS_to_TTTs.
+ smt(n_gt0 size_ge0).
+move=> x xs IH; elim => //=.
+ rewrite flatten_nil flatten_cons -size_eq0 size_cat size_SSS_to_TTTs.
+ smt(n_gt0 size_ge0).
+move=> y ys IH2.
+rewrite !flatten_cons eqseq_cat ?size_SSS_to_TTTs //=; move => [/SSS_to_TTTs_inj -> /= ?].
+by apply IH.
+qed.
+
+lemma SSS_from_TTTs_nseq0 k:
+ 0 <= k <= n =>
+ SSS_from_TTTs (nseq k dTTT) = dSSS.
+proof.
+move=> Hk; apply SSS_to_TTTs_inj.
+rewrite SSS_to_TTTs_nil SSS_from_TTTsK ?size_nseq 1:/# ler_maxr 1:/#.
+by rewrite cat_nseq /#.
+qed.
+
+lemma SSSs_from_TTTs_nseq0 k:
+ 0 <= k =>
+ SSSs_from_TTTs (nseq k dTTT) = nseq (k %/ n + b2i (! n %| k)) dSSS.
+proof.
+admit.
+qed.
+
+lemma chunkfill_SSSs_from_TTTs k z l:
+ chunkfill dSSS k (SSSs_from_TTTs (l ++ nseq z dTTT))
+ = chunkfill dSSS k (SSSs_from_TTTs l).
+proof.
+admit.
+qed.
+
+lemma SSSs_to_TTTs_take k l:
+ SSSs_to_TTTs (take k l)
+ = take (n*k) (SSSs_to_TTTs l).
+proof.
+elim/natind: k l => //=.
+ move=> k Hk l; rewrite !take_le0 //.
+ by apply StdOrder.IntOrder.mulr_ge0_le0; smt(n_gt0).
+move=> k Hk IH [|x xs] //=.
+have ->/=: ! (k+1 <= 0) by rewrite -ltzNge ltzS.
+rewrite !SSSs_to_TTTs_cons take_cat.
+have ->/=: ! (n * (k + 1) < size (SSS_to_TTTs x)).
+ by rewrite size_SSS_to_TTTs; smt(n_gt0).
+by rewrite mulzDr /= IH size_SSS_to_TTTs /#.
+qed.
+
+lemma SSSs_to_TTTs_drop k l:
+ SSSs_to_TTTs (drop k l)
+ = drop (n*k) (SSSs_to_TTTs l).
+proof.
+elim/natind: k l => //=.
+ move=> k Hk l; rewrite !drop_le0 //.
+ smt(n_gt0).
+move=> k Hk IH [|x xs] //=.
+have ->/=: ! (k+1 <= 0) by rewrite -ltzNge ltzS.
+rewrite !SSSs_to_TTTs_cons drop_cat.
+have ->/=: ! (n * (k + 1) < size (SSS_to_TTTs x)).
+ by rewrite size_SSS_to_TTTs; smt(n_gt0).
+by rewrite mulzDr /= IH size_SSS_to_TTTs /#.
+qed.
+
+lemma SSSs_to_TTTs_map2 fS' fT' l1 l2:
+ (forall x1 x2, SSS_to_TTTs (fS' x1 x2)
+ = map2 fT' (SSS_to_TTTs x1) (SSS_to_TTTs x2)) =>
+ SSSs_to_TTTs (JUtils.map2 fS' l1 l2)
+ = map2 fT' (SSSs_to_TTTs l1) (SSSs_to_TTTs l2).
+proof.
+move => Hfg.
+elim: l2 l1 => //=.
+ by move=> [|x xs]; rewrite SSSs_to_TTTs_nil // SSSs_to_TTTs_cons /= map2_nilr /#.
+move=> y ys IH1; elim => //=.
+ by rewrite SSSs_to_TTTs_cons /SSSs_to_TTTs flatten_nil map2_nill.
+move=> x xs IH2.
+rewrite !SSSs_to_TTTs_cons map2_cat.
+ by rewrite !size_SSS_to_TTTs.
+rewrite IH1; congr.
+by apply Hfg.
+qed.
+
+lemma SSSs_from_TTTs_nil: SSSs_from_TTTs [] = [].
+proof. by rewrite /SSSs_from_TTTs chunkify_nil. qed.
+
+lemma SSSs_from_TTTs_cat l1 l2:
+ n %| size l1 =>
+ SSSs_from_TTTs (l1++l2)
+ = SSSs_from_TTTs l1 ++ SSSs_from_TTTs l2.
+proof. by move=> Hsz; rewrite /SSSs_from_TTTs chunkify_cat ?n_gt0 // !map_cat. qed.
+
+lemma SSSs_from_TTTs_cons l:
+ 0 < size l =>
+ SSSs_from_TTTs l = SSS_from_TTTs (take n l) :: SSSs_from_TTTs (drop n l).
+proof.
+move: n_gt0 => n_gt0 Hsz0.
+by rewrite /SSSs_from_TTTs chunkify_cons //.
+qed.
+
+lemma size_SSSs_from_TTTs l:
+ size (SSSs_from_TTTs l)
+ = size l %/ n + b2i (! n %| size l).
+proof.
+rewrite /gL size_map size_chunkify //.
+by apply n_gt0.
+qed.
+
+lemma SSSs_from_TTTsK l:
+ SSSs_to_TTTs (SSSs_from_TTTs l)
+ = chunkfill dTTT n l.
+proof.
+rewrite /SSSs_to_TTTs /SSSs_from_TTTs -map_comp.
+apply map_chunkifyK; first exact n_gt0.
+move=> xs Hxs; rewrite /(\o) SSS_from_TTTsK //.
+admitted (*
+rewrite take_cat ifF 1:/# take_nseq.
+smt(size_ge0).
+qed.
+*).
+
+lemma SSSs_from_TTTsK_dvd l:
+ n %| size l => SSSs_to_TTTs (SSSs_from_TTTs l) = l.
+proof.
+move=> Hn; rewrite /SSSs_from_TTTs chunkify_chunk ?n_gt0 // /SSSs_to_TTTs -map_comp.
+apply map_chunkK => //; first exact n_gt0.
+by move=> xs Hxs; rewrite /(\o) SSS_from_TTTsK 1:/# Hxs /= nseq0 cats0.
+qed.
+
+lemma SSSs_to_TTTsK:
+ cancel SSSs_to_TTTs SSSs_from_TTTs.
+proof.
+move=> k; apply SSSs_to_TTTs_inj.
+rewrite SSSs_from_TTTsK_dvd // size_SSSs_to_TTTs dvdz_mulr.
+smt(n_gt0).
+qed.
+
+lemma SSSs_to_TTTs_nseq0 k:
+ SSSs_to_TTTs (nseq k dSSS) = nseq (n*k) dTTT.
+proof.
+elim/natind: k => /=.
+ by move=> k Hk1; rewrite !nseq0_le //; smt(n_gt0).
+move=> k Hk IH; rewrite nseqS // SSSs_to_TTTs_cons IH //.
+rewrite addzC mulzDr mulz1 nseq_add //; first 2 smt(n_gt0).
+by rewrite SSS_to_TTTs_nil.
+qed.
+
+lemma nth_SSSs_to_TTTs l i:
+ 0 <= i < n*size l =>
+ nth dTTT (SSSs_to_TTTs l) i
+ = nth dTTT (SSS_to_TTTs (nth dSSS l (i %/ n))) (i %% n).
+proof.
+move=> Hi; rewrite /SSSs_to_TTTs (nth_flatten _ n).
+ rewrite allP; move=> x /mapP [y [Hy ->]] /=.
+ by rewrite size_SSS_to_TTTs.
+rewrite (nth_map dSSS) //.
+apply divz_cmp => //; first by apply n_gt0.
+by rewrite mulzC.
+qed.
+
+lemma drop_SSSs_from_TTTs k l:
+ drop k (SSSs_from_TTTs l)
+ = SSSs_from_TTTs (drop (n*k) l).
+proof.
+have n_gt0:= n_gt0.
+rewrite /SSSs_from_TTTs -map_drop; congr.
+by apply drop_chunkify.
+qed.
+
+lemma take_SSSs_from_TTTs k l:
+ take k (SSSs_from_TTTs l)
+ = SSSs_from_TTTs (take (n*k) l).
+proof.
+have n_gt0 := n_gt0.
+rewrite /SSSs_from_TTTs -map_take; congr.
+by apply take_chunkify.
+qed.
+
+lemma nth_SSSs_from_TTTs l k:
+  0 <= k =>
+  nth dSSS (SSSs_from_TTTs l) k
+  = SSS_from_TTTs (take n (drop (n*k) l)).
+proof.
+have n_gt0 Hk0 := n_gt0.
+rewrite /SSSs_from_TTTs (nth_map' []) /=.
+ by rewrite SSS_from_TTTs_nil.
+by congr; rewrite nth_chunkify //.
+qed.
+
+(*
+lemma chunkify_SSSs_from_TTTs k l:
+ chunkify k (SSSs_from_TTTs l)
+ = map SSSs_from_TTTs (chunkify (k*n) l).
+proof.
+rewrite /SSSs_from_TTTs /chunkify /=.
+print map_comp.
+rewrite -map_comp.
+rewrite map_mkseq /(\o) /=.
+congr.
+ apply fun_ext => x.
+ rewrite map_mkseq /(\o) /=.
+rewrite -/(mkseq (fun (x0 : int) => SSS_from_TTTs (take n (drop (n * x0) l))) (size l %/ n + b2i (! n %| size l))).
+rewrite drop_mkseq.
+ admit.
+rewrite take_mkseq /=.
+ admit.
+congr.
+ apply fun_ext => y.
+admit.
+admit.
+
+rewrite !size_map !size_iota !lez_maxr.
+smt. 
+case: (n %| size l) => C1 /=.
+ rewrite !b2i0 /=.
+ admit.
+rewrite !b2i1.
+admit.
+qed.
+*)
+
+end ListEmbedding.
+
+
+
+clone export ListEmbedding as Bytes2Bits
+ with
+ type SSS <- W8.t,
+ type TTT <- bool,
+ op n <- 8,
+ op dSSS <- W8.zero,
+ op dTTT <- false,
+ op SSS_to_TTTs <- W8.w2bits,
+ op SSS_from_TTTs <- W8.bits2w
+ rename [op, lemma]
+  "SSSs_to_TTTs" as "bytes_to_bits"
+  "SSSs_from_TTTs" as "bytes_from_bits"
+  "SSS_to_TTTs" as "byte_to_bits"
+  "SSS_from_TTTs" as "byte_from_bits"
+  "SSSs" as "bytes"
+  "SSS" as "byte"
+  "TTT" as "bit"
+  proof n_gt0 by done
+  proof *.
+realize size_byte_to_bits by done.
+realize byte_to_bits_inj by apply W8.w2bits_inj.
+realize byte_to_bitsK by apply W8.w2bitsK.
+realize byte_to_bits_nil by rewrite /w2bits -mkseq_nseq /mkseq -iotaredE /=.
+realize byte_from_bits_nil by apply W8_bits2w_nil.
+realize byte_from_bitsK by apply W8_bits2wK'.
+
+clone export ListEmbedding as W64s2Bits
+ with
+ type SSS <- W64.t,
+ type TTT <- bool,
+ op n <- 64,
+ op dSSS <- W64.zero,
+ op dTTT <- false,
+ op SSS_to_TTTs <- W64.w2bits,
+ op SSS_from_TTTs <- W64.bits2w
+ rename [op, lemma]
+  "SSSs_to_TTTs" as "w64L_to_bits"
+  "SSSs_from_TTTs" as "w64L_from_bits"
+  "SSS_to_TTTs" as "w64_to_bits"
+  "SSS_from_TTTs" as "w64_from_bits"
+  "SSSs" as "w64L"
+  "SSS" as "w64"
+  "TTT" as "bit"
+  proof n_gt0 by done
+  proof *.
+realize size_w64_to_bits by done.
+realize w64_to_bits_inj by apply W64.w2bits_inj.
+realize w64_to_bitsK by apply W64.w2bitsK.
+realize w64_to_bits_nil by rewrite /w2bits -mkseq_nseq /mkseq -iotaredE /=.
+realize w64_from_bits_nil by apply W64_bits2w_nil.
+realize w64_from_bitsK by apply W64_bits2wK'.
+
+
+
+
+
+clone export ListEmbedding as W64s2Bytes
+ with
+ type SSS <- W64.t,
+ type TTT <- W8.t,
+ op n <- 8,
+ op dSSS <- W64.zero,
+ op dTTT <- W8.zero,
+ op SSS_to_TTTs <- W8u8.to_list,
+ op SSS_from_TTTs <- W8u8.pack8
+ rename [op, lemma]
+  "SSSs_to_TTTs" as "w64L_to_bytes"
+  "SSSs_from_TTTs" as "w64L_from_bytes"
+  "SSS_to_TTTs" as "w64_to_bytes"
+  "SSS_from_TTTs" as "w64_from_bytes"
+  "SSSs" as "w64L"
+  "SSS" as "w64"
+  "TTT" as "byte"
+  proof n_gt0 by done
+  proof *.
+realize size_w64_to_bytes by done.
+realize w64_to_bytes_inj by apply W8u8_to_list_inj.
+realize w64_to_bytesK by apply W8u8_to_listK.
+realize w64_to_bytes_nil by rewrite /= !W8u8.get_zero -mkseq_nseq /mkseq -iotaredE /=. 
+realize w64_from_bytesK by apply W8u8_to_list_pack8.
+realize w64_from_bytes_nil by apply W8u8_pack8_nil.
+
+
+lemma w64_to_bytes_to_bits w:
+ bytes_to_bits (W8u8.to_list w) = W64.w2bits w.
+proof.
+by rewrite /bytes_to_bits /w2bits /(\bits8) /flatten /mkseq -iotaredE /=.
+qed.
+
+lemma w64L_to_bytes_to_bits l:
+ bytes_to_bits (w64L_to_bytes l) = w64L_to_bits l.
+proof.
+elim: l; first by rewrite /w64L_to_bytes /flatten.
+move=> x xs IH.
+by rewrite /w64L_to_bytes map_cons flatten_cons w64L_to_bits_cons -IH bytes_to_bits_cat  w64_to_bytes_to_bits //. 
+qed.
+
+(*
+print map_comp.
+print chunkify.
+search mkseq.
+
+lemma bits2bytes2w64s l:
+ w64L_from_bytes (bits2bytes l)
+ = w64L_from_bits l.
+admitted.
+
+map w64_from_bytes (chunkify 8 (bits2bytes l))
+= map (w64_from_bytes \o bits2bytes) (chunkify 64 l)
+= map w64_from_bytes (map bits2bytes (chunkify 64 l))
+
+ou seja:
+chunkify k (bits2bytes l)
+= map bits2bytes (chunkify (k*8) l)
+
+mkseq (fun i => mkseq (fun k => ) sl)
+= mkseq (
+*)
+
+(*
+lemma nosmt size_ind ['a] (P : 'a list -> bool):
+ (forall xs, (forall l, size l < size xs => P l) => P xs) => forall l, P l.
+proof.
+move=> H.
+have Hind: forall (xs l:'a list), size l <= size xs => P l.
+ elim => //=.
+  smt.
+ move=> xs Hxs l Hl.
+ apply H => *. smt.
+by move=> l; apply (Hind l).
+qed.
+*)
+
+
+
+(*
 (*******************************************************************************)
-(*                                   W8 lists                                  *)
+(*                             W8 lists (aka "bytes")                          *)
 (*******************************************************************************)
 
-op w8L2bits (l: W8.t list) : bool list =
+type bits = bool list.
+type bytes = W8.t list.
+
+op bytes2bits (l: bytes) : bits =
  flatten (map W8.w2bits l).
 
-lemma w8L2bits_nil: w8L2bits [] = [] by done.
+lemma bytes2bits_nil: bytes2bits [] = [] by done.
 
-hint simplify w8L2bits_nil.
+hint simplify bytes2bits_nil.
 
-lemma w8L2bits_cons x xs: w8L2bits (x::xs) = W8.w2bits x ++ w8L2bits xs.
-proof. by rewrite /w8L2bits map_cons flatten_cons. qed.
+lemma bytes2bits_cons x xs:
+ bytes2bits (x::xs) = W8.w2bits x ++ bytes2bits xs.
+proof. by rewrite /bytes2bits map_cons flatten_cons. qed.
 
-lemma w8L2bits_cat l1 l2:
- w8L2bits (l1++l2) = w8L2bits l1 ++ w8L2bits l2.
-proof. by elim: l1 => //= x xs IH; rewrite !w8L2bits_cons IH catA. qed.
+lemma bytes2bits_cat l1 l2:
+ bytes2bits (l1++l2) = bytes2bits l1 ++ bytes2bits l2.
+proof. by elim: l1 => //= x xs IH; rewrite !bytes2bits_cons IH catA. qed.
 
-lemma size_w8L2bits x:
- size (w8L2bits x) = 8 * size x.
+lemma size_bytes2bits x:
+ size (bytes2bits x) = 8 * size x.
 proof.
-by rewrite /w8L2bits size_flatten -map_comp /(\o) /= StdBigop.Bigint.sumzE
+by rewrite /bytes2bits size_flatten -map_comp /(\o) /= StdBigop.Bigint.sumzE
 StdBigop.Bigint.BIA.big_mapT /(\o) /= StdBigop.Bigint.big_constz count_predT_eq.
 qed.
 
-(*hint simplify size_w8L2bits.*)
+(*hint simplify size_bytes2bits.*)
 
-lemma take_w8L2bits n l:
- take (8*n) (w8L2bits l) = w8L2bits (take n l).
+lemma take_bytes2bits n l:
+ take (8*n) (bytes2bits l) = bytes2bits (take n l).
 proof.
 elim/natind: n l => //=.
  move=> n Hn l; rewrite !take_le0 //.
  by apply StdOrder.IntOrder.mulr_ge0_le0.
 move=> n Hn IH [|x xs] //=.
 have ->/=: ! (n+1 <= 0) by rewrite -ltzNge ltzS.
-rewrite !w8L2bits_cons take_cat.
+rewrite !bytes2bits_cons take_cat.
 have ->/=: ! (8 * (n + 1) < size (w2bits x)) by rewrite W8.size_w2bits /#.
 by rewrite mulzDr /= IH.
 qed.
 
-lemma drop_w8L2bits n l:
- drop (8*n) (w8L2bits l) = w8L2bits (drop n l).
+lemma drop_bytes2bits n l:
+ drop (8*n) (bytes2bits l) = bytes2bits (drop n l).
 proof.
 elim/natind: n l => //=.
  move=> n Hn l; rewrite !drop_le0 //.
  by apply StdOrder.IntOrder.mulr_ge0_le0.
 move=> n Hn IH [|x xs] //=.
 have ->/=: ! (n+1 <= 0) by rewrite -ltzNge ltzS.
-rewrite !w8L2bits_cons drop_cat.
+rewrite !bytes2bits_cons drop_cat.
 have ->/=: ! (8 * (n + 1) < size (w2bits x)) by rewrite W8.size_w2bits /#.
 by rewrite mulzDr /= IH.
 qed.
 
-lemma w8L2bits_u64 w: w8L2bits (W8u8.to_list w) = W64.w2bits w.
+lemma bytes2bits_u64 w: bytes2bits (W8u8.to_list w) = W64.w2bits w.
 proof.
-by rewrite /w8L2bits /w2bits /(\bits8) /flatten /mkseq -iotaredE /=.
+by rewrite /bytes2bits /w2bits /(\bits8) /flatten /mkseq -iotaredE /=.
 qed.
 
-op bits2w8L (bs: bool list) : W8.t list =
- map W8.bits2w (BitEncoding.BitChunking.chunk 8 (chunkfill false 8 bs)).
+op bits2bytes (bs: bits) : bytes =
+ map W8.bits2w (chunkify 8 bs).
 
-lemma bits2w8L_nil: bits2w8L [] = [].
+lemma bits2bytes_nil: bits2bytes [] = [].
+proof. by rewrite /bits2bytes /chunkify /chunk /= mkseq0. qed.
+
+hint simplify bits2bytes_nil.
+
+lemma size_bits2bytes bs:
+ size (bits2bytes bs)
+ = size bs %/ 8 + b2i (! 8 %| size bs).
+proof. by rewrite /bits2bytes size_map size_chunkify //. qed.
+
+lemma bits2bytesK bs:
+ 8 %| size bs => bytes2bits (bits2bytes bs) = bs.
 proof.
-rewrite /bits2w8L chunkfill_nil.
-by rewrite /BitEncoding.BitChunking.chunk /= mkseq0.
+move=> Hsz; rewrite /bytes2bits /bits2bytes chunkify_chunk //.
+rewrite -map_comp map_chunkK //.
+by move=> l Hl; rewrite /(\o) bits2wK //.
 qed.
 
-hint simplify bits2w8L_nil.
-
-lemma size_bits2w8L' bs:
- size (bits2w8L bs) = (size bs - 1) %/ 8 + 1.
+lemma bits2bytesK' bs:
+ bytes2bits (bits2bytes bs)
+ = bs ++ chunkfill bs 8 false.
 proof.
-rewrite /bits2w8L size_map BitEncoding.BitChunking.size_chunk //.
-rewrite size_chunkfill //.
-rewrite {3}(:8 = 1*8) 1:/# -mulzDl.
-by rewrite -(addz0 (((size bs - 1) %/ 8 + 1) * 8)) divzMDl.
+rewrite /bytes2bits /bits2bytes -map_comp.
+apply map_chunkifyK => //.
+move=> l Hl @/(\o).
+case: (size l = 8) => C.
+ by rewrite bits2wK // take_size_cat //.
+rewrite -(W8_bits2w_cat_nseq0 l (8-size l)). 
+rewrite bits2wK ?size_cat ?size_nseq 1:/# take_cat ifF 1:/# take_nseq lez_minl //.
+smt(size_ge0).
 qed.
 
-lemma size_bits2w8L bs:
- 8 %| size bs => size (bits2w8L bs) = size bs %/ 8.
-proof. by rewrite dvdzP size_bits2w8L' => [[k ->]]; smt(). qed.
-
-lemma bits2w8LK bs:
- 8 %| size bs => w8L2bits (bits2w8L bs) = bs.
+lemma bytes2bits_inj: injective bytes2bits.
 proof.
-move=> Hsz.
-rewrite /w8L2bits -map_comp dvd_chunkfill //.
-have : forall (x : bool list),
-        x \in BitEncoding.BitChunking.chunk 8 bs =>
-         idfun x = W8.w2bits (W8.bits2w x).
- move=> x Hx; beta.
- rewrite W8.bits2wK //.
- by apply (BitEncoding.BitChunking.in_chunk_size _ _ _ _ Hx).
-rewrite List.eq_in_map => <-.
-by rewrite map_id BitEncoding.BitChunking.chunkK // Hsz.
-qed.
-
-lemma bits2w8LK' bs:
- w8L2bits (bits2w8L bs) = chunkfill false 8 bs.
-proof.
-rewrite /bits2w8L -chunkfillK //.
-by rewrite bits2w8LK ?chunkfillP // chunkfillK.
-qed.
-
-lemma w8L2bits_inj: injective w8L2bits.
-proof.
-rewrite /w8L2bits; elim.
+rewrite /bytes2bits; elim.
  move=> [|y ys] //=.
  rewrite flatten_nil flatten_cons.
  rewrite eq_sym -size_eq0 size_cat size_w2bits.
@@ -124,36 +1008,51 @@ rewrite !flatten_cons eqseq_cat //=; move => [/W8.w2bits_inj -> /= ?].
 by apply IH.
 qed.
 
-lemma w8L2bitsK: cancel w8L2bits bits2w8L.
+lemma bytes2bitsK: cancel bytes2bits bits2bytes.
 proof.
-move=> k; apply w8L2bits_inj.
-by rewrite bits2w8LK // size_w8L2bits dvdz_mulr.
+move=> k. apply bytes2bits_inj.
+by rewrite bits2bytesK // size_bytes2bits dvdz_mulr.
 qed.
 
-lemma w8L2bits_xor l1 l2:
- w8L2bits (JUtils.map2 W8.(`^`) l1 l2)
- = map2 Bool.(^^) (w8L2bits l1) (w8L2bits l2).
+(*
+lemma bytes2bits_xor' l1 l2:
+ JUtils.map2 W8.(`^`) l1 l2
+ = bits2w8L (map2 Bool.(^^) (bytes2bits l1) (bytes2bits l2)).
+proof.
+admit.
+qed.
+*)
+
+from Jasmin require import JUtils.
+
+lemma bytes2bits_xor l1 l2:
+ bytes2bits (JUtils.map2 W8.(`^`) l1 l2)
+ = map2 Bool.(^^) (bytes2bits l1) (bytes2bits l2).
 proof.
 elim: l1 l2 => //=.
- move=> [|y ys]; rewrite w8L2bits_nil // w8L2bits_cons.
+ move=> [|y ys]; rewrite bytes2bits_nil // bytes2bits_cons.
  by rewrite map2C /= /#.
 move=> x xs IH1; elim => //=.
  rewrite map2C; first by move=> b1 b2; ring.
- by rewrite w8L2bits_cons map2C /= /#.
+ by rewrite bytes2bits_cons map2C /= /#.
 move=> y ys IH2.
-rewrite !w8L2bits_cons map2_cat.
+rewrite !bytes2bits_cons map2_cat.
  by rewrite !size_w2bits.
 rewrite IH1; congr.
 by rewrite W8.xorE map2_w2bits_w2bits.
+(*
+rewrite bytes2bits_xor' bits2w8LK //.
+rewrite size_map2 !size_bytes2bits /#.
+*)
 qed.
 
-lemma w8L2bits_nseq0 n:
+lemma bytes2bits_nseq0 n:
  0 <= n =>
- w8L2bits (nseq n W8.zero) = nseq (8*n) false.
+ bytes2bits (nseq n W8.zero) = nseq (8*n) false.
 proof.
 elim/natind: n => /=.
  by move=> n Hn1 Hn2; rewrite !nseq0_le 1,2:/#.
-move=> n Hn IH H; rewrite nseqS // w8L2bits_cons IH //.
+move=> n Hn IH H; rewrite nseqS // bytes2bits_cons IH //.
 rewrite addzC mulzDr mulz1 nseq_add // 1:/#; congr.
 by rewrite /w2bits -mkseq_nseq /mkseq -iotaredE /=.
 qed.
@@ -163,67 +1062,61 @@ qed.
 (*                                   W64 lists                                  *)
 (*******************************************************************************)
 
-op w64L2bits (l: W64.t list) : bool list =
+type w64 = W64.t.
+type w64s = w64 list.
+
+op w64s2bits (l: w64s) : bits =
  flatten (map W64.w2bits l).
 
-lemma size_w64L2bits l:
- size (w64L2bits l) = 64 * size l.
+lemma size_w64s2bits l:
+ size (w64s2bits l) = 64 * size l.
 proof.
-by rewrite /w64L2bits size_flatten -map_comp /(\o) /= StdBigop.Bigint.sumzE
+by rewrite /w64s2bits size_flatten -map_comp /(\o) /= StdBigop.Bigint.sumzE
 StdBigop.Bigint.BIA.big_mapT /(\o) /= StdBigop.Bigint.big_constz count_predT_eq.
 qed.
 
 (*hint simplify size_w64L2bits.*)
 
-op bits2w64L (bs: bool list) : W64.t list =
- map W64.bits2w (BitEncoding.BitChunking.chunk 64 (chunkfill false 64 bs)).
+op bits2w64s (bs: bits) : w64s =
+ map W64.bits2w (chunkify 64 bs).
 
-lemma bits2w64L_nil: bits2w64L [] = [].
+lemma bits2w64s_nil: bits2w64s [] = [].
 proof.
-rewrite /bits2w64L chunkfill_nil.
-by rewrite /BitEncoding.BitChunking.chunk /= mkseq0.
+by rewrite /bits2w64s /chunkify /chunk /= mkseq0.
 qed.
 
-lemma size_bits2w64L' bs:
- size (bits2w64L bs) = (size bs - 1) %/ 64 + 1.
+lemma size_bits2w64s' bs:
+ size (bits2w64s bs)
+ = size bs %/ 64 + b2i (! 64 %| size bs).
+proof. by rewrite /bits2w64s size_map size_chunkify //. qed.
+
+hint simplify bits2w64s_nil.
+
+lemma bits2w64sK bs:
+ 64 %| size bs => w64s2bits (bits2w64s bs) = bs.
 proof.
-rewrite /bits2w64L size_map BitEncoding.BitChunking.size_chunk //.
-rewrite size_chunkfill //.
-rewrite {3}(:64 = 1*64) 1:/# -mulzDl.
-by rewrite -(addz0 (((size bs - 1) %/ 64 + 1) * 64)) divzMDl.
+move=> Hsz; rewrite /w64s2bits /bits2w64s chunkify_chunk //.
+rewrite -map_comp map_chunkK //.
+by move=> l Hl; rewrite /(\o) bits2wK //.
 qed.
 
-lemma size_bits2w64L bs:
- 64 %| size bs => size (bits2w64L bs) = size bs %/ 64.
-proof. by rewrite dvdzP size_bits2w64L' => [[k ->]]; smt(). qed.
-
-hint simplify bits2w64L_nil.
-
-lemma bits2w64LK bs:
- 64 %| size bs => w64L2bits (bits2w64L bs) = bs.
+lemma bits2w64sK' bs:
+ w64s2bits (bits2w64s bs)
+ = bs ++ chunkfill bs 64 false.
 proof.
-move=> Hsz.
-rewrite /w64L2bits -map_comp dvd_chunkfill //.
-have : forall (x : bool list),
-        x \in BitEncoding.BitChunking.chunk 64 bs =>
-         idfun x = (fun x => w2bits ((bits2w x))%W64) x.
- move=> x Hx; beta.
- rewrite W64.bits2wK //.
- by apply (BitEncoding.BitChunking.in_chunk_size _ _ _ _ Hx).
-rewrite List.eq_in_map => <-.
-by rewrite map_id BitEncoding.BitChunking.chunkK // Hsz.
+rewrite /w64s2bits /bits2w64s -map_comp.
+apply map_chunkifyK => //.
+move=> l Hl @/(\o).
+case: (size l = 64) => C.
+ by rewrite bits2wK // take_size_cat //.
+rewrite -(W64_bits2w_cat_nseq0 l (64-size l)). 
+rewrite bits2wK ?size_cat ?size_nseq 1:/# take_cat ifF 1:/# take_nseq lez_minl //.
+smt(size_ge0).
 qed.
 
-lemma bits2w64LK' bs:
- w64L2bits (bits2w64L bs) = chunkfill false 64 bs.
+lemma w64s2bits_inj: injective w64s2bits.
 proof.
-rewrite /bits2w64L -chunkfillK //.
-by rewrite bits2w64LK ?chunkfillP // chunkfillK.
-qed.
-
-lemma w64L2bits_inj: injective w64L2bits.
-proof.
-rewrite /w64L2bits; elim.
+rewrite /w64s2bits; elim.
  move=> [|y ys] //=.
  rewrite flatten_nil flatten_cons.
  rewrite eq_sym -size_eq0 size_cat size_w2bits.
@@ -239,78 +1132,78 @@ move=> [/W64.w2bits_inj <- /= ?].
 by apply IH.
 qed.
 
-lemma w64L2bitsK: cancel w64L2bits bits2w64L.
+lemma w64s2bitsK: cancel w64s2bits bits2w64s.
 proof.
-move=> k; apply w64L2bits_inj.
-by rewrite bits2w64LK // size_w64L2bits dvdz_mulr.
+move=> k; apply w64s2bits_inj.
+by rewrite bits2w64sK // size_w64s2bits dvdz_mulr.
 qed.
 
-lemma w64L2bits_nil: w64L2bits [] = [] by done.
+lemma w64s2bits_nil: w64s2bits [] = [] by done.
 
-lemma w64L2bits_cons x xs: w64L2bits (x::xs) = W64.w2bits x ++ w64L2bits xs.
-proof. by rewrite /w64L2bits map_cons flatten_cons. qed.
+lemma w64s2bits_cons x xs: w64s2bits (x::xs) = W64.w2bits x ++ w64s2bits xs.
+proof. by rewrite /w64s2bits map_cons flatten_cons. qed.
 
-lemma w64L2bits_cat l1 l2:
- w64L2bits (l1++l2) = w64L2bits l1 ++ w64L2bits l2.
+lemma w64s2bits_cat l1 l2:
+ w64s2bits (l1++l2) = w64s2bits l1 ++ w64s2bits l2.
 proof.
 elim: l1 => //=.
-by move=> x xs IH; rewrite !w64L2bits_cons IH -!catA; congr.
+by move=> x xs IH; rewrite !w64s2bits_cons IH -!catA; congr.
 qed.
 
-lemma take_w64L2bits n l:
- take (64*n) (w64L2bits l) = w64L2bits (take n l).
+lemma take_w64s2bits n l:
+ take (64*n) (w64s2bits l) = w64s2bits (take n l).
 proof.
 elim/natind: n l => //=.
  move=> n Hn l; rewrite !take_le0 //.
  by apply StdOrder.IntOrder.mulr_ge0_le0.
 move=> n Hn IH [|x xs] /=.
- by rewrite w64L2bits_nil.
+ by rewrite w64s2bits_nil.
 have ->/=: ! (n+1 <= 0) by rewrite -ltzNge ltzS.
-rewrite !w64L2bits_cons take_cat.
+rewrite !w64s2bits_cons take_cat.
 have ->/=: ! (64 * (n + 1) < size (w2bits x)) by rewrite W64.size_w2bits /#.
 by rewrite mulzDr /= IH.
 qed.
 
-lemma drop_w64L2bits n l:
- drop (64*n) (w64L2bits l) = w64L2bits (drop n l).
+lemma drop_w64s2bits n l:
+ drop (64*n) (w64s2bits l) = w64s2bits (drop n l).
 proof.
 elim/natind: n l => //=.
  move=> n Hn l; rewrite !drop_le0 //.
  by apply StdOrder.IntOrder.mulr_ge0_le0.
 move=> n Hn IH [|x xs] /=.
- by rewrite w64L2bits_nil.
+ by rewrite w64s2bits_nil.
 have ->/=: ! (n+1 <= 0) by rewrite -ltzNge ltzS.
-rewrite !w64L2bits_cons drop_cat.
+rewrite !w64s2bits_cons drop_cat.
 have ->/=: ! (64 * (n + 1) < size (w2bits x)) by rewrite W64.size_w2bits /#.
 by rewrite mulzDr /= IH.
 qed.
 
-lemma nth_w64L2bits l i:
+lemma nth_w64s2bits l i:
  0 <= i < 64 * size l =>
- nth false (w64L2bits l) i
+ nth false (w64s2bits l) i
  = nth false (W64.w2bits (nth W64.zero l (i %/ 64))) (i%%64).
 proof.
-move=> Hi; rewrite /w64L2bits (BitEncoding.BitChunking.nth_flatten _ 64).
+move=> Hi; rewrite /w64s2bits (nth_flatten _ 64).
  by rewrite allP; move=> x /mapP [y [Hy ->]].
 rewrite (nth_map W64.zero) //.
 apply divz_cmp => //.
 by rewrite mulzC.
 qed.
 
-lemma w64L2bits_xor l1 l2:
- w64L2bits (JUtils.map2 W64.(`^`) l1 l2)
- = map2 Bool.(^^) (w64L2bits l1) (w64L2bits l2).
+lemma w64s2bits_xor l1 l2:
+ w64s2bits (JUtils.map2 W64.(`^`) l1 l2)
+ = map2 Bool.(^^) (w64s2bits l1) (w64s2bits l2).
 proof.
 elim: l1 l2 => //=.
- move=> [|y ys]; rewrite w64L2bits_nil // w64L2bits_cons.
+ move=> [|y ys]; rewrite w64s2bits_nil // w64s2bits_cons.
  rewrite map2C /=.
   exact W64.xorwC.
  smt().
 move=> x xs IH1; elim => //=.
- rewrite w64L2bits_nil map2C; first by move=> b1 b2; ring.
- rewrite w64L2bits_cons map2C /#.
+ rewrite w64s2bits_nil map2C; first by move=> b1 b2; ring.
+ rewrite w64s2bits_cons map2C /#.
 move=> y ys IH2.
-rewrite !w64L2bits_cons map2_cat.
+rewrite !w64s2bits_cons map2_cat.
  by rewrite !size_w2bits.
 rewrite IH1; congr.
 by rewrite W64.xorE map2_w2bits_w2bits.
@@ -318,11 +1211,11 @@ qed.
 
 lemma w64L2bits_nseq0 n:
  0 <= n =>
- w64L2bits (nseq n W64.zero) = nseq (64*n) false.
+ w64s2bits (nseq n W64.zero) = nseq (64*n) false.
 proof.
 elim/natind: n => /=.
- by move=> n Hn1 Hn2; rewrite !nseq0_le 1,2:/# w64L2bits_nil.
-move=> n Hn IH H; rewrite nseqS // w64L2bits_cons IH //.
+ by move=> n Hn1 Hn2; rewrite !nseq0_le 1,2:/# w64s2bits_nil.
+move=> n Hn IH H; rewrite nseqS // w64s2bits_cons IH //.
 rewrite addzC mulzDr mulz1 nseq_add // 1:/#; congr.
 by rewrite /w2bits -mkseq_nseq /mkseq -iotaredE /=.
 qed.
@@ -331,26 +1224,28 @@ qed.
 (*                      W8 lists  =>  W64 lists                                *)
 (*******************************************************************************)
 
-op w8L2w64L (l: W8.t list) : W64.t list =
- map W8u8.pack8 (BitEncoding.BitChunking.chunk 8 (chunkfill W8.zero 8 l)).
+op bytes2w64s (l: bytes) : w64s =
+ map W8u8.pack8 (chunkify 8 l).
 
-lemma w8L2w64L_nil: w8L2w64L [] = [].
-proof. by rewrite /w8L2w64L chunkfill_nil /BitEncoding.BitChunking.chunk mkseq0. qed.
+lemma bytes2w64s_nil: bytes2w64s [] = [].
+proof. by rewrite /bytes2w64s /chunkify /chunk mkseq0. qed.
 
-hint simplify w8L2w64L_nil.
+hint simplify bytes2w64s_nil.
 
-lemma w8L2w64L_cat l1 l2:
- 8 %| size l1 => w8L2w64L (l1++l2) = w8L2w64L l1 ++ w8L2w64L l2.
+lemma size_bytes2w64s l:
+ size (bytes2w64s l)
+ = size l %/ 8 + b2i (! 8 %| size l).
+proof. by rewrite /bytes2w64s size_map size_chunkify //. qed.
+
+lemma bytes2w64s_cat l1 l2:
+ 8 %| size l1 => bytes2w64s (l1++l2) = bytes2w64s l1 ++ bytes2w64s l2.
+proof. by move=> Hsz; rewrite /bytes2w64s chunkify_cat // !map_cat. qed.
+
+(*
+lemma bytes2w64s_singl xs:
+ 0 < size xs <= 8 => bytes2w64s xs = [pack8 xs].
 proof.
-move=> Hsz; rewrite /w8L2w64L chunkfill_cat //.
-rewrite BitEncoding.BitChunking.chunk_cat // map_cat.
-by rewrite (chunkfillK' l1) //.
-qed.
-
-lemma w8L2w64L_singl xs:
- 0 < size xs <= 8 => w8L2w64L xs = [pack8 xs].
-proof.
-move=> Hsz; rewrite /w8L2w64L /BitEncoding.BitChunking.chunk.
+move=> Hsz; rewrite /bytes2w64s /chunkify /chunk.
 have ->: size (chunkfill W8.zero 8 xs) %/ 8 = 1.
  rewrite size_chunkfill // /#.
 rewrite mkseq1 /= drop0 take_oversize.
@@ -358,76 +1253,90 @@ rewrite mkseq1 /= drop0 take_oversize.
 rewrite !pack8E; apply W64.init_ext => x Hx /=.
 by congr; rewrite !W8u8.Pack.get_of_list 1,2:/# nth_chunkfill.
 qed.
+*)
 
-lemma w8L2w64L_cons l:
- 0 < size l =>
- w8L2w64L l = W8u8.pack8 (take 8 l) :: w8L2w64L (drop 8 l).
+lemma chunk0 ['a] n (l: 'a list):
+ size l < n =>
+ chunk n l = [].
 proof.
-move=> Hsz0; rewrite -{1}(cat_take_drop 8 l).
-case: (size l <= 8) => Hsz.
- by rewrite !drop_oversize //= cats0 take_oversize // w8L2w64L_singl // E /=.
-rewrite w8L2w64L_cat.
- by rewrite size_take // (: 8 < size l) 1:/# /= dvdzz.
-by rewrite w8L2w64L_singl // size_take // /#.
+move=> Hl; rewrite /chunk divz_small; smt(size_ge0 mkseq0).
 qed.
 
-lemma drop_w8L2w64L n l:
- drop n (w8L2w64L l) = w8L2w64L (drop (8*n) l).
+lemma bytes2w64s_cons l:
+ 0 < size l =>
+ bytes2w64s l = W8u8.pack8 (take 8 l) :: bytes2w64s (drop 8 l).
+proof.
+move=> Hsz0.
+ rewrite -{1}(cat_take_drop 8 l).
+case: (size l < 8) => Hsz.
+ by rewrite !drop_oversize 1:/# cats0 take_oversize 1:/# bytes2w64s_nil /bytes2w64s chunkifyE // chunk0 /#.
+by rewrite bytes2w64s_cat ?size_take 1..2:/# {1}/bytes2w64s chunkify_chunk // ?size_take // 1:/# chunk1 /#.
+qed.
+
+lemma drop_bytes2w64s n l:
+ drop n (bytes2w64s l) = bytes2w64s (drop (8*n) l).
 proof.
 elim/natind: n l => //=.
  by move=> n Hn l; rewrite !drop_le0 // /#.
 move=> n Hn IH l.
 rewrite -drop_drop //.
 move: l => [|x xs] //.
-rewrite {1}(w8L2w64L_cons (x::xs) _) /=; first smt(size_ge0).
+rewrite {1}(bytes2w64s_cons (x::xs) _) /=; first smt(size_ge0).
 rewrite drop0 (:! 8 * (n + 1) <= 0) 1:/# /= IH drop_drop 1:/# //.
 by congr; congr; ring.
 qed.
 
-lemma size_w8L2w64L l:
- size (w8L2w64L l) = (size l - 1) %/ 8 + 1.
-proof.
-rewrite /w8L2w64L size_map BitEncoding.BitChunking.size_chunk //.
-rewrite size_chunkfill //. 
-by rewrite -{3}(mul1z 8) -mulzDl mulzK.
-qed.
+(*
+lemma size_bytes2w64L' l:
+ 8 %| size l => size (bytes2w64L l) = size l %/ 8.
+proof. by rewrite size_bytes2w64L dvdz_eq => E; smt(). qed.
+*)
 
-lemma size_w8L2w64L' l:
- 8 %| size l => size (w8L2w64L l) = size l %/ 8.
-proof. by rewrite size_w8L2w64L dvdz_eq => E; smt(). qed.
-
-lemma take_w8L2w64L n l:
- take n (w8L2w64L l) = w8L2w64L (take (8*n) l).
+lemma take_bytes2w64s n l:
+ take n (bytes2w64s l) = bytes2w64s (take (8*n) l).
 proof.
 rewrite -{1}(cat_take_drop (8*n) l).
 case: (0 <= 8*n) => Hsz0; last by rewrite !take_le0 /#.
 case: (8*n <= size l) => E.
- rewrite w8L2w64L_cat.
-  rewrite size_take' 1:/# E /= /#.
- rewrite take_cat' !size_w8L2w64L size_take' // !E /=.
- rewrite (:n <= (8 * n - 1) %/ 8 + 1) 1:/# /= take_oversize //.
- by rewrite size_w8L2w64L size_take' // E /= /#.
+ rewrite bytes2w64s_cat.
+  by rewrite size_take' 1:/# E /= /#.
+ rewrite take_cat' !size_bytes2w64s size_take' // !E /= ifT. 
+  by rewrite (:8 %| 8 * n) /#.
+ rewrite take_oversize // size_bytes2w64s !size_take //.
+ case: (8*n < size l) => C; smt().
 rewrite drop_oversize 1:/# cats0 take_oversize //.
-by rewrite size_w8L2w64L size_take' /#.
+by rewrite size_bytes2w64s size_take' /#.
 qed.
 
-lemma nth_w8L2w64L (l : W8.t list) (i : int):
-  nth W64.zero (w8L2w64L l) i
-  = pack8_t (W8u8.Pack.init (fun j => l.[8*i + j])).
+lemma nth_map' ['a 'b] (da: 'a) (f: 'a -> 'b) (l: 'a list) db i:
+ f da = db =>
+ nth db (map f l) i = f (nth da l i).
 proof.
-rewrite /w8L2w64L.
-case: (0 <= i /\ i < (size l-1) %/ 8 + 1) => E; last first.
- rewrite nth_out; first by rewrite size_map size_chunkfilled /#.
- rewrite -(W8u8.Pack.init_ext (fun j => W8.zero)).
- move=> j Hj /=; rewrite nth_out// 1:/#.
- rewrite -(W8u8.unpack8K W64.zero); congr.
- apply W8u8.Pack.ext_eq => j Hj.
- by rewrite !W8u8.Pack.initiE //= unpack8E initiE //= get_zero.
-rewrite (nth_map []) /=; first by rewrite size_chunkfilled /#.
-rewrite nth_chunkfilled' // 1:/#.
-congr; apply W8u8.Pack.ext_eq => j Hj.
-rewrite W8u8.Pack.initiE //=.
-by rewrite W8u8.Pack.get_of_list //= nth_mkseq //.
+move => Hf.
+case: (0 <= i && i < size l) => C.
+ by rewrite (nth_map da) //.
+by rewrite !nth_out; smt(size_map).
+qed.
+
+lemma pack8_nil: W8u8.pack8 [] = W64.zero.
+proof.
+rewrite pack8E W8u8.Pack.of_listE.
+rewrite -(W8u8.Pack.init_ext (fun j => W8.zero)) //=.
+apply W64.ext_eq => k Hk; rewrite initiE //=.
+by rewrite W8u8.Pack.initiE 1:/# /=.
+qed.
+
+lemma nth_bytes2w64s (l : bytes) (i : int):
+  0 <= i =>
+  nth W64.zero (bytes2w64s l) i
+  = pack8 (take 8 (drop (8*i) l)).
+(*
+  = pack8_t (W8u8.Pack.init (fun j => l.[8*i + j])).*)
+proof.
+move=> Hi; rewrite /bytes2w64s (nth_map' []) /=.
+ exact pack8_nil.
+congr; apply W8u8.Pack.ext_eq => k Hk.
+by rewrite !get_of_list //= nth_chunkify //.
 qed.
 
 
@@ -436,61 +1345,61 @@ qed.
 (*******************************************************************************)
 
 
-op w64L2w8L (l: W64.t list) : W8.t list =
+op w64s2bytes (l: w64s) : bytes =
  flatten (map W8u8.to_list l).
 
-lemma w64L2w8L_nil:
- w64L2w8L [] = [].
-proof. by rewrite /w64L2w8L. qed.
+lemma w64s2bytes_nil:
+ w64s2bytes [] = [].
+proof. by rewrite /w64s2bytes. qed.
 
-hint simplify w64L2w8L_nil.
+hint simplify w64s2bytes_nil.
 
-lemma w64L2w8L_cons x xs:
- w64L2w8L (x::xs) = W8u8.to_list x ++ w64L2w8L xs.
-proof. by rewrite /w64L2w8L map_cons flatten_cons. qed.
+lemma w64s2bytes_cons x xs:
+ w64s2bytes (x::xs) = W8u8.to_list x ++ w64s2bytes xs.
+proof. by rewrite /w64s2bytes map_cons flatten_cons. qed.
 
-lemma size_w64L2w8L (l: W64.t list):
- size (w64L2w8L l) = 8 * size l.
+lemma size_w64s2bytes (l: W64.t list):
+ size (w64s2bytes l) = 8 * size l.
 proof.
 elim: l => //= x xs IH.
-by rewrite w64L2w8L_cons size_cat IH /#.
+by rewrite w64s2bytes_cons size_cat IH /#.
 qed.
 
-(*hint simplify size_w64L2w8L.*)
+(*hint simplify size_w64s2bytes.*)
 
-lemma w64L2w8L2bits l:
- w8L2bits (w64L2w8L l) = w64L2bits l.
+lemma w64s2bytes2bits l:
+ bytes2bits (w64s2bytes l) = w64s2bits l.
 proof.
-elim: l; first by rewrite /w64L2w8L /flatten.
+elim: l; first by rewrite /w64s2bytes /flatten.
 move=> x xs IH.
-by rewrite /w64L2w8L map_cons flatten_cons w64L2bits_cons -IH w8L2bits_cat  w8L2bits_u64 //. 
+by rewrite /w64s2bytes map_cons flatten_cons w64s2bits_cons -IH bytes2bits_cat  bytes2bits_u64 //. 
 qed.
 
-lemma w64L2w8L_singl x: w64L2w8L [x] = W8u8.to_list x by rewrite /w64L2w8L.
+lemma w64s2bytes_singl x: w64s2bytes [x] = W8u8.to_list x by rewrite /w64s2bytes.
 
-lemma w64L2w8L_cat l1 l2:
- w64L2w8L (l1++l2) = w64L2w8L l1 ++ w64L2w8L l2.
+lemma w64s2bytes_cat l1 l2:
+ w64s2bytes (l1++l2) = w64s2bytes l1 ++ w64s2bytes l2.
 proof.
 by elim: l1 => //= x xs IH.
 qed.
 
-lemma take_w64L2w8L n l:
- take (8*n) (w64L2w8L l) = w64L2w8L (take n l).
+lemma take_w64s2bytes n l:
+ take (8*n) (w64s2bytes l) = w64s2bytes (take n l).
 proof.
 elim: l n => //= x xs IH n.
 case: (n <= 0) => E /=; first by rewrite take_le0 /#.
-by rewrite !w64L2w8L_cons -IH take_cat /= ifF /#.
+by rewrite !w64s2bytes_cons -IH take_cat /= ifF /#.
 qed.
 
-lemma nth_w64L2w8L (l : W64.t list) (i : int):
-  nth W8.zero (w64L2w8L l) i
+lemma nth_w64s2bytes (l : W64.t list) (i : int):
+  nth W8.zero (w64s2bytes l) i
   = nth W64.zero l (i %/ 8) \bits8 (i %% 8).
 proof.
-rewrite /w64L2w8L.
+rewrite /w64s2bytes.
 have Hsz: all (fun (s : W8.t list) => size s = 8)
               (map (fun (w : W64.t) => (to_list w)%W8u8) l).
  by rewrite allP => x /mapP [y [Hy ->]].
-rewrite (BitEncoding.BitChunking.nth_flatten W8.zero 8) //.
+rewrite (nth_flatten W8.zero 8) //.
 move: Hsz; rewrite allP => Hsz.
 case: (0 <= i %/ 8 < size l) => E; last first.
  rewrite nth_out; first rewrite nth_out ?size_map /#.
@@ -498,13 +1407,39 @@ case: (0 <= i %/ 8 < size l) => E; last first.
 by rewrite (nth_map W64.zero) //= /#.
 qed.
 
-lemma w8L2w64LK (l: W8.t list):
- 8 %| size l => w64L2w8L (w8L2w64L l) = l.
-proof.
+print pack8K.
+
+lemma to_list_pack8 (bs: bytes):
+ size bs <= 8 =>
+ W8u8.to_list (pack8 bs) = bs.
 move=> Hsz.
-rewrite /w64L2w8L /w8L2w64L -map_comp dvd_chunkfill //.
+rewrite /= !pack8bE // !get_of_list //.
+admit.
+qed.
+
+print "_.[_]".
+search pack8_t (\bits8).
+
+lemma bytes2w64sK (l: W8.t list):
+ 8 %| size l => w64s2bytes (bytes2w64s l) = l.
+proof.
+move=> Hsz; rewrite /bytes2w64s /w64s2bytes chunkify_chunk //.
+rewrite -map_comp map_chunkK //.
+move=> xs Hxs; rewrite /(\o).
+print pack8K.
+rewrite -(W8u8.pack8K).
+print W8u8.pack8.
+print W8u8.Pack.of_listK.
+print W8u8.to_list.
+print pack8K.
+print pack8.
+print W8u8.pack8K.
+ /=. smt. bits2wK //.
+qed.
+move=> Hsz.
+rewrite /w64s2bytes /bytes2w64s -map_comp dvd_chunkfill //.
 have : forall (x : W8.t list),
-        x \in BitEncoding.BitChunking.chunk 8 l =>
+        x \in chunk 8 l =>
          idfun x = W8u8.to_list (pack8 x).
  move=> x Hx; rewrite /idfun /= /=.
  have x_size:= (BitEncoding.BitChunking.in_chunk_size _ _ _ _ Hx) => //.
@@ -513,11 +1448,11 @@ rewrite List.eq_in_map => <-.
 by rewrite map_id BitEncoding.BitChunking.chunkK // Hsz.
 qed.
 
-lemma w8Lw64LK' l:
- w64L2w8L (w8L2w64L l) = chunkfill W8.zero 8 l.
+lemma bytesw64sK' l:
+ w64s2bytes (bytes2w64s l) = chunkfill W8.zero 8 l.
 proof.
-rewrite /w8L2w64L -chunkfillK //.
-by rewrite w8L2w64LK ?chunkfillP // chunkfillK.
+rewrite /bytes2w64s -chunkfillK //.
+by rewrite bytes2w64sK ?chunkfillP // chunkfillK.
 qed.
 
 lemma W8u8_to_listE (w: W64.t):
@@ -543,9 +1478,9 @@ proof.
 by move=> w1 w2; rewrite !W8u8_to_listE => /W8u8.Pack.to_list_inj /W8u8_unpack8_inj.
 qed.
 
-lemma w64L2w8L_inj: injective w64L2w8L.
+lemma w64s2bytes_inj: injective w64s2bytes.
 proof.
-rewrite /w64L2w8L; elim.
+rewrite /w64s2bytes; elim.
  by move=> [|y ys].
 move=> x xs IH; elim => //.
 move=> y ys IH2.
@@ -554,11 +1489,14 @@ rewrite eqseq_cat //; beta.
 by move => [/W8u8_to_list_inj -> ?]; congr; last by apply IH.
 qed.
 
-lemma w64L2w8LK: cancel w64L2w8L w8L2w64L.
+lemma w64s2bytesK: cancel w64s2bytes bytes2w64s.
 proof.
-move=> k; apply w64L2w8L_inj.
-by rewrite w8L2w64LK // size_w64L2w8L dvdz_mulr.
+move=> k; apply w64s2bytes_inj.
+by rewrite bytes2w64sK // size_w64s2bytes dvdz_mulr.
 qed.
+*)
+
+
 
 (*******************************************************************************)
 (*                          MEMORY OPERATIONS                                  *)
@@ -661,14 +1599,18 @@ lemma stores64_rcons mem out xs x:
  = storeW64 (stores64 mem out xs) (out + 8*size xs) x.
 proof. by rewrite -cats1 stores64_cat. qed.
 
+lemma w64L_to_bytes_singl x:
+ w64L_to_bytes [x]
+ = W8u8.to_list x by done.
+
 lemma stores64_stores8 mem out l:
- stores64 mem out l = stores8 mem out (w64L2w8L l).
+ stores64 mem out l = stores8 mem out (w64L_to_bytes l).
 proof.
 rewrite stores8E; elim/last_ind: l mem out => //=.
  by move=> mem out; rewrite store0.
 move=> xs x IH mem out.
-rewrite stores64_rcons IH -cats1 w64L2w8L_cat stores_cat w64L2w8L_singl.
-by rewrite stores_u64 size_w64L2w8L.
+rewrite stores64_rcons IH -cats1 w64L_to_bytes_cat stores_cat /=  w64L_to_bytes_singl.
+by rewrite stores_u64 size_w64L_to_bytes.
 qed.
 
 
@@ -741,12 +1683,13 @@ qed.
 
 lemma nth_memread_u64 mem in_ inlen i:
  0 <= i => 8*i+8 <= inlen =>
- loadW64 mem (in_+8*i) = nth W64.zero (w8L2w64L (memread mem in_ inlen)) i.
+ loadW64 mem (in_+8*i) = nth W64.zero (w64L_from_bytes (memread mem in_ inlen)) i.
 proof.
-move=> ??; rewrite nth_w8L2w64L.
+move=> ??; rewrite nth_w64L_from_bytes 1:/#.
 rewrite /loadW64 W8u8.pack8E pack8E; apply W64.init_ext => x Hx /=.
-congr; rewrite W8u8.Pack.initiE 1:/# /= /memread.
-by rewrite W8u8.Pack.initiE 1:/# /= nth_mkseq /#.
+congr; rewrite W8u8.Pack.initiE 1:/# /= /memread /=.
+rewrite of_listE W8u8.Pack.initiE 1:/# /=.
+by rewrite drop_mkseq 1:/# take_mkseq 1:/# /= nth_mkseq /#.
 qed.
 
 
@@ -784,24 +1727,25 @@ lemma nth_memread64 m a sz i:
 proof. by move=> Hsz; rewrite nth_mkseq //. qed.
 
 lemma memread64E m a sz:
- memread64 m a sz = w8L2w64L (memread m a (8*sz)).
+ memread64 m a sz = w64L_from_bytes (memread m a (8*sz)).
 proof.
 apply (eq_from_nth W64.zero).
- by rewrite size_mkseq size_w8L2w64L size_mkseq /#. 
+ by rewrite size_mkseq size_w64L_from_bytes size_mkseq /#. 
 rewrite size_mkseq => i Hi.
-rewrite nth_w8L2w64L nth_memread64 1:/# /loadW64; congr.
+rewrite nth_w64L_from_bytes 1:/# nth_memread64 1:/# /loadW64 of_listE; congr.
 apply W8u8.Pack.init_ext => j Hj /=.
-by rewrite nth_mkseq /#.
+rewrite drop_memread 1:/# take_memread 1:/# nth_mkseq /#.
 qed.
 
 lemma memread_split64 mem a sz:
  0 <= sz =>
  memread mem a sz
- = w64L2w8L (memread64 mem a (sz %/ 8))
+ = w64L_to_bytes (memread64 mem a (sz %/ 8))
    ++ memread mem (a + sz %/8 * 8) (sz %% 8).
 proof.
 move=> Hsz; rewrite (memread_split (sz %/ 8*8)) 1:/#; congr.
- by rewrite memread64E w8L2w64LK ?size_memread /#.
+ rewrite memread64E w64L_from_bytesK chunkfillE //. (* /chunkify_fillsuffix.*)
+ by rewrite size_memread 1:/# /= dvdz_mulr 1:dvdzz /#.
 by rewrite modzE.
 qed.
 
