fips202/properties/Keccak1600_Spec.ec
@@ -3,10 +3,17 @@
 
    Properties of the Keccak1600 specification.
 
+    - function byte-based specification
+    - correctness wrt imperative spec [FIPS202_SHA3.ec]
+
 ******************************************************************************)
 require import AllCore List Int IntDiv.
+
 require StdOrder.
 import StdOrder.IntOrder.
+
+require BitEncoding.
+import BitEncoding.BitChunking.
 
 require export FIPS202_SHA3.
 
@@ -14,26 +21,19 @@ require import Keccakf1600_Spec.
 
 import EclibExtra.
 
-require BitEncoding.
-import BitEncoding.BitChunking.
+(*
 
+type bit = bool.
+type bits = bool list.
+*)
 type byte = W8.t.
 type bytes = W8.t list.
-type w64 = W64.t.
-type w64s = W64.t list.
-
-(** sets a specific byte of a 64-bit word *)
-op w64_set_u8 (w: w64, pos: int, x: byte): w64 =
- pack8_t (unpack8 w).[pos <- x].
-
-op w64_xor_u8 (w: w64, pos: int, x: byte): w64 =
- let w8u8 = unpack8 w in pack8_t w8u8.[pos <- w8u8.[pos] `^` x].
 
 op bytes2state (bs: bytes): state =
- Array25.of_list W64.zero (w8L2w64L bs).
+ Array25.of_list W64.zero (w64L_from_bytes bs).
 
 op state2bytes (st: state): bytes =
- w64L2w8L (to_list st).
+ w64L_to_bytes (to_list st).
 
 op state_set_u8 (st: state, pos: int, x: byte): state =
  st.[pos %/ 8 <- w64_set_u8 st.[pos %/ 8] (pos %% 8) x].
@@ -52,18 +52,18 @@ op state_absorb (st: state, m: bytes): state =
 op state_squeeze (st: state, len: int): bytes =
  take len (state2bytes st).
 
-
+(*
 
 (** [chunkremnant] returns the leftovers not handled by [chunk] *)
 op chunkremnant ['a] (n: int) (bs: 'a list) =
  drop (size bs %/ n * n) bs.
-
+*)
 
 abbrev KECCAK_F1600 = keccak_f1600_op.
 
 (** absorb intermediate blocks *)
-op state_absorb_iblocks (r64: int, m: bytes): state =
- foldl (fun st m => KECCAK_F1600 (state_absorb st m)) st0 (chunk (8*r64) m).
+op state_absorb_iblocks (ml: bytes list): state =
+ foldl (fun st m => KECCAK_F1600 (state_absorb st m)) st0 ml.
 
 (** [addratebit] flips the "rate bit" *)
 op addratebit (r64: int, st: state): state =
@@ -78,8 +78,8 @@ op addratebit (r64: int, st: state): state =
 op keccak1600_absorb_op (r64: int, suffix: byte, m: bytes): state =
  addratebit
   r64
-  (state_absorb (state_absorb_iblocks r64 m)
-                (rcons (chunkremnant (8*r64) m) suffix)).
+  (state_absorb (state_absorb_iblocks (chunk (8*r64) m))
+                (rcons (chunkremains (8*r64) m) suffix)).
 
 
 (** squeezes [len] bytes from [KECCAK_F1600^i(st)] *)
@@ -113,10 +113,338 @@ op SHAKE128 (m: bytes, len8: int): bytes =
 op SHAKE256 (m:bytes, len8: int): bytes =
  keccak1600_op 17 (W8.of_int 31) m len8.
 
+(** Using XOFs without explicit output len argument.
+
+    Citation from [FIPS-202, A-2 (pag. 24)]:
+
+    "By design, the output length for an XOF does not affect the bits
+    that it produces, which means that the output length is not a
+    necessary input to the function. Conceptually, the output can be
+    an infinite string, and the application/protocol/system that
+    invokes the function simply computes the desired number of initial
+    bits of that string. Consequently, when two different output
+    lengths are chosen for a common message, the two outputs are
+    closely related: the longer output is an extension of the shorter
+    output. For example, given any positive integers "d" and "e", and any
+    message "M", "Trunc_d(SHAKE128(M, d+e))" is identical to "SHAKE128(M,
+    d)". The same property holds for SHAKE256."
+
+    To support such a use, we provide functions returning the "ith" (i \in
+    [1..]) block of SHAKE128/256 for a given input.                                   *)
+
+op SHAKE128_i (m: bytes, i: int): bytes =
+ drop (8*21*(i-1)) (SHAKE128 m (8*21*i)).
+
+op SHAKE256_i (m: bytes, i: int): bytes =
+ drop (8*17*(i-1)) (SHAKE256 m (8*17*i)).
 
 
 
-(** [SHAKE128_i(m,i)] returns the last 168 bytes of [SHAKE128(m,i*168)] (ith block) *)
-op SHAKE128_i (m: bytes) (i: int): bytes =
- drop (168*(i-1)) (SHAKE128 m (i*168)).
+
+
+
+(*******************************************************************************
+                               Correctness proof
+*******************************************************************************)
+
+
+lemma Array25_of_listK' ['a] (d:'a) l:
+ to_list (Array25.of_list d l)
+ = take 25 (l ++ nseq 25 d).
+proof.
+apply (eq_from_nth d).
+ by rewrite size_to_list size_take; smt(size_cat size_ge0 size_nseq).
+rewrite size_to_list => i Hi.
+rewrite /Array25.to_list nth_mkseq //=.
+rewrite get_of_list // take_cat.
+case: (25 < size l) => C.
+ by rewrite nth_take /#.
+rewrite nth_cat.
+case: (i < size l) => C2 //.
+by rewrite take_nseq nth_nseq; smt(nth_out size_ge0).
+qed.
+
+print chunkfill.
+(* este faz sentido (em vez de ter de lidar com os nseqs... *)
+op chunkfill' ['a] (d:'a) n l =
+ take n (l ++ nseq n d).
+
+
+lemma state2bitsK:
+ cancel state2bits bits2state.
+admitted.
+
+lemma bits2stateK bs:
+ state2bits (bits2state bs)
+ = chunkfill' false 1600 bs.
+ admitted.
+
+lemma addstateA (s1 s2 s3: state):
+ addstate s1 (addstate s2 s3) = addstate (addstate s1 s2) s3.
+proof.
+rewrite /addstate; apply ext_eq => i Hi.
+by rewrite !map2iE // W64.WRing.AddMonoid.addmA. 
+qed.
+
+op xorbits (xs ys: bool list) = map2 Logic.(^) xs ys.
+
+lemma addstate_xorbits bs1 bs2:
+ size bs1 = size bs2 =>
+ addstate (bits2state bs1) (bits2state bs2)
+ = bits2state (xorbits bs1 bs2).
+proof.
+move=> Hsz .
+rewrite /bits2state /addstate; apply Array25.ext_eq => i Hi.
+rewrite map2iE // !get_of_list //.
+rewrite !nth_w64L_from_bits /xorbits 1..3:/#  drop_map2 take_map2.
+apply W64.ext_eq => k Hk.
+rewrite !get_bits2w //.
+case: (k < size (take 64 (drop (i * 64) bs1))) => C.
+ rewrite (nth_map2 false false).
+  rewrite size_take // size_drop 1:/#.
+  smt(size_take size_drop size_ge0).
+ smt(W64.get_bits2w).
+rewrite nth_out; first by rewrite size_map2 1:/#.
+by rewrite xorwE !get_bits2w // !nth_take 1..4:/# !nth_drop 1..4:/# !nth_out; smt(size_take size_drop).
+qed.
+
+lemma W64_bits2w_nseq0 n:
+ W64.bits2w (nseq n false)
+ = W64.zero.
+proof.
+apply W64.ext_eq => i Hi.
+by rewrite /bits2w initiE //= nth_nseq_if /#.
+qed.
+
+lemma addratebit_addstate r64 st:
+ 0 < r64 <= 25 =>
+ addratebit r64 st
+ = addstate st (bits2state (rcons (nseq (64*r64-1) false) true)).
+proof.
+move=> Hr64; rewrite /addratebit /addstate /=.
+apply ext_eq => i Hi.
+rewrite map2iE //.
+case: (i = r64-1) => C; last first.
+ rewrite get_setE 1:/# C /= /bits2state get_of_list //.
+ rewrite nth_w64L_from_bits 1:/# -cats1.
+ case (i < r64-1) => C2.
+  rewrite drop_cat size_nseq ifT 1:/# drop_nseq 1:/#.
+  rewrite take_cat ifT ?size_nseq 1:/# take_nseq. 
+  by rewrite W64_bits2w_nseq0 /#.
+ rewrite drop_cat ifF ?size_nseq 1:/# drop_oversize 1:/#.
+ by rewrite /= W64_bits2w_nil.
+rewrite /bits2state get_of_list // nth_w64L_from_bits 1:/# -cats1.
+rewrite get_setE 1:/# ifT 1:/#.
+apply W64.ext_eq => k Hk.
+rewrite xorwE /=.
+case: (k = 63) => C2.
+ rewrite /w64_xor_u8 /= pack8wE // get_setE // C2 /=.
+ rewrite nth_take // nth_drop // 1:/# nth_cat ifF.
+  by rewrite size_nseq /#.
+ rewrite size_nseq C /= lez_maxr 1:/# of_intE /int2bs /mkseq -iotaredE /=.
+ pose X:= (_ = 0).
+ by have ->{X}/=: X=true by smt().
+rewrite /w64_xor_u8 /= pack8wE // get_setE // eq_sym.
+rewrite C drop_cat ifT ?size_nseq 1:/# drop_nseq 1:/#.
+rewrite take_cat ?size_nseq ifF 1:/#.
+pose X:= 64 - _.
+have ->{X}: X=(size [true]) by smt().
+rewrite take_size get_bits2w 1:// nth_cat ifT ?size_nseq 1:/# nth_nseq 1:/# /=.
+case: (k %/ 8 = 7) => E.
+ rewrite W8u8.get_bits8 // E xorwE.
+ have Emod: k %% 8 <> 7 by smt().
+ have ->: (W8.of_int 128).[k %% 8] = false.
+  by rewrite of_intE /int2bs /mkseq -iotaredE /= /bits2w initiE 1:/# /= /#.
+ smt().
+by rewrite get_unpack8 1:/# W8u8.get_bits8.
+qed.
+
+lemma size_pad10star1 r len:
+ 0 < r =>
+ 0 <= len %% r <= r-2 =>
+ size (pad10star1 r len)
+ = r - (len %% r).
+proof.
+move=> Hr Hlen.
+rewrite /pad10star1 /= size_rcons size_nseq lez_maxr 1:/#.
+rewrite -modzDml -modzNm -modzDl /#.
+qed.
+
+(*
+lemma size_pad10star1 r len:
+ 0 < r =>
+ 0 <= len <= r-2 =>
+ size (pad10star1 r len)
+ = r - (len %% r).
+proof.
+move=> Hr Hlen.
+by rewrite /pad10star1 /= size_rcons size_nseq lez_maxr /#.
+qed.
+*)
+
+lemma nosmt pad10star1_modr r64 len8 mbits_size:
+ 0 < r64 =>
+ pad10star1 (64*r64) (8*len8 + mbits_size)
+ = pad10star1 (64*r64) (8 * (len8 %% (8*r64)) + mbits_size).
+proof.
+move=> Hr; rewrite /pad10star1; congr; congr; congr.
+have ->: -(8 * len8 + mbits_size) - 2 = - (8 * len8 + (mbits_size + 2)) by ring.
+rewrite -modzNm -modzDml {1}(:64*r64=8*(8*r64)) 1:/# -mulz_modr // modzNm /#.
+qed.
+
+lemma nosmt chunk_padded r64 bs mbits:
+ 0 < r64 =>
+ size mbits <= 6 =>
+ chunk (64*r64) (bytes_to_bits bs ++ mbits ++ pad10star1 (64*r64) (8*size bs + size mbits))
+ = chunk (64*r64) (bytes_to_bits bs)
+   ++ [chunkremains (64*r64) (bytes_to_bits bs) ++ mbits ++ pad10star1 (64*r64) (8*(size bs%%(8*r64)) + size mbits)].
+proof.
+move => Hr64 Hmbits; rewrite -catA chunk_cat' 1:/#; congr.
+rewrite chunk1 1:/#.
+ rewrite !size_cat size_chunkremains size_bytes_to_bits size_pad10star1 1:/#; first smt(size_ge0).
+ rewrite (:64*r64=8*r64*8) 1:/#.
+ have [_ B]:= divmod_mul (8*r64) 8 (size bs) (size mbits) _ _; smt(size_ge0).
+by rewrite !catA; congr; congr; apply pad10star1_modr.
+qed.
+
+(*
+search chunkremains.
+lemma chunkify_cat' ['a]:
+   forall (n : int) (l1 l2 : 'a list),
+     0 < n =>
+     chunkify n (l1 ++ l2) = chunk n l1 ++ chunkify n (chunkremains n l1 ++ l2).
+*)
+(*
+lemma chunk_padded' r64 bs mbits:
+ 0 < r64 =>
+ size mbits <= 6 =>
+ chunk (64*r64) (bytes_to_bits bs ++ mbits ++ pad10star1 (64*r64) (8*size bs + size mbits))
+ = chunk (64*r64) (bytes_to_bits bs)
+   ++ [chunkremains (64*r64) (bytes_to_bits bs) ++ mbits ++ pad10star1 (64*r64) (8*size bs + size mbits)].
+proof.
+move => Hr64 Hmbits; rewrite -catA chunk_cat' 1:/#; congr.
+rewrite chunk1 1:/#.
+ rewrite !size_cat size_chunkremains size_bytes_to_bits size_pad10star1 1:/#; first smt(size_ge0).
+ rewrite (:64*r64=8*r64*8) 1:/#.
+ have [_ B]:= divmod_mul (8*r64) 8 (size bs) (size mbits) _ _; smt(size_ge0).
+smt(catA).
+qed.
+*)
+
+lemma pad10star1_split r l n:
+ 0 < r =>
+ size l <= r-2 =>
+ n = size  l =>
+ l ++ pad10star1 r n
+ = xorbits (rcons l true ++ nseq (r - size l - 1) false)
+           (rcons (nseq (r-1) false) true).
+proof.
+have Hsz_ge0 := size_ge0 <:bool>.
+move => Hr Hsz ->; apply (eq_from_nth false).
+ by rewrite size_map2 !size_cat !size_rcons !size_nseq size_pad10star1 /#.
+move=> i.
+pose S:= size _; have ->{S}: S = r. 
+ rewrite /S size_cat size_pad10star1 // 2:/#.
+ by rewrite modz_small /#.
+move=> Hi.
+rewrite /xorbits (nth_map2 false false).
+ smt(size_rcons size_nseq size_cat).
+rewrite nth_cat.
+case: (i < size l) => C1.
+ rewrite -cats1 -!catA nth_cat C1 /= nth_rcons ifT.
+  by rewrite size_nseq /#.
+ by rewrite nth_nseq /#.
+rewrite -cats1 -catA nth_cat C1.
+rewrite /pad10star1 /=.
+case: (i-size l<>0) => C2 /=.
+ rewrite nth_nseq 1:/# addFb nth_rcons.
+ have ->: ((- size l)-2) %% r = r-size l-2.
+  by rewrite -modzDl /#.
+ rewrite size_nseq lez_maxr 1:/#.
+ case: (i - size l - 1 < r - size l - 2) => C3;
+  smt(nth_nseq nth_rcons size_nseq).
+rewrite nth_rcons nth_nseq; smt(size_nseq size_ge0).
+qed.
+
+(*
+op keccak1600_absorb_op (r64: int, suffix: byte, m: bytes): state =
+ addratebit
+  r64
+  (state_absorb (state_absorb_iblocks r64 m)
+                (rcons (chunkremains (8*r64) m) suffix)).
+*)
+lemma bits2state_cat_nseq0 n bs:
+ bits2state (bs ++ nseq n false) = bits2state bs.
+proof.
+rewrite /bits2state.
+admit.
+qed.
+
+lemma bits2bytes2state bs:
+ bits2state bs = bytes2state (bytes_from_bits bs).
+admitted.
+
+lemma addstate_last (st:state) r64 mbits bs suffix:
+ 0 < r64 <= 25 =>
+ size mbits <= 6 =>
+ suffix = W8.bits2w (rcons mbits true) =>
+ addstate st (bits2state (chunkremains (64*r64) (bytes_to_bits bs) ++ mbits ++ pad10star1 (64*r64) (8*(size bs %% (8*r64)) + size mbits)))
+ = addratebit r64 (addstate st (bytes2state (rcons (chunkremains (8*r64) bs) suffix))).
+proof.
+move=> Hr64 Hmbits Hsuffix.
+rewrite pad10star1_split 1:/#.
+  by rewrite size_cat size_chunkremains size_bytes_to_bits /#.
+ by rewrite size_cat size_chunkremains size_bytes_to_bits /#.
+rewrite -addstate_xorbits. 
+ rewrite size_cat !size_rcons !size_cat !size_nseq size_chunkremains size_bytes_to_bits; smt(size_ge0).
+rewrite addstateA -addratebit_addstate //; congr; congr.
+rewrite bits2state_cat_nseq0 -(bits2state_cat_nseq0 (7-size mbits)) bits2bytes2state.
+pose L := _ ++ _.
+have ->: L = bytes_to_bits (rcons (chunkremains (8 * r64) bs) suffix).
+ rewrite /L -!cats1 bytes_to_bits_cat /chunkremains bytes_to_bits_drop -!catA; congr.
+  by congr; rewrite size_bytes_to_bits /#.
+ rewrite !catA bytes_to_bits_cons bytes_to_bits_nil cats0.
+ rewrite Hsuffix W8_bits2wK' ?size_rcons 1:/# cats1; congr; smt().
+by rewrite bytes_to_bitsK.
+qed.
+
+
+lemma nth_chunk ['a] k (l: 'a list) i:
+ 0 < k =>
+ k %| size l =>
+ nth [] (chunk k l) i =
+ take k (drop (k*i) l).
+proof.
+admitted.
+
+
+print Keccak1600.
+(*
+  proc sponge1600_pad10star1(r : int, m : bool list, d : int) : bool list = {
+*)
+
+
+lemma sponge_correct _r64 _m _suffix _mbits _len8:
+ 0 < _len8 => (* this can be removed by an extra case... *)
+ size _mbits <= 6 =>
+ W8.w2bits _suffix = rcons _mbits true =>
+ hoare [ Keccak1600.sponge1600_pad10star1:
+         r = 64*_r64 /\ m = bytes_to_bits _m ++ _mbits /\ d = 8*_len8
+         ==> res = bytes_to_bits (keccak1600_op _r64 _suffix _m _len8 )].
+proof.
+move=> Hlen8 Hmbits Hsuffix; proc; simplify.
+seq 6: (#pre /\ s = keccak1600_absorb_op _r64 _suffix _m).
+print keccak1600_absorb_op.
+ while (#pre /\ n = size m %/ 8 + 1 /\ 0 <= i <= n /\
+        pl = chunk r (bytes_to_bits _m ++ _mbits ++ pad10star1 r (8 * (size _m) + size _mbits)) /\
+        s <- state_absorb_iblocks r64 
+ admit.
+exlim (keccak1600_absorb_op _r64 _suffix _m) => st.
+splitwhile 2: (size z + d < d).
+seq 2: (#[:-2]pre /\ s = (iter (d %/ r) KECCAK_F1600 st) /\ size z = r * (d %/ r)) => //.
+ admit.
+admit.
+qed.
+
+
 
